refine tarai

coq/tarai.v
@@ -29,40 +29,38 @@ Definition ntarai3v (n : nat) (av bv cv : Z):=
 ntarai3 n (Some av) (Some bv) (Some cv). 
 
 Inductive Tarai_value:
-     nat -> option Z -> option Z -> option Z -> Z -> Prop :=
-| Tarai_a_le_b n (av bv: Z) c (Hle: av <= bv):
-     Tarai_value n (Some av) (Some bv) c bv
-| Tarai_a_gt_b_1 n (av bv cv: Z) (v1 v2: Z)
-     (Hgt: av > bv)
+     nat -> Z -> Z -> Z -> Z -> Prop :=
+| Tarai_a_le_b n a b c (Hle: a <= b):
+     Tarai_value n a b c b
+| Tarai_a_gt_b_1 n a b c v1 v2
+     (Hgt: a > b)
      (Hle2: v1 <= v2)
-     (Hrec1: Tarai_value n (Some (av-1)) (Some bv) (Some cv) v1)
-     (Hrec2: Tarai_value n (Some (bv-1)) (Some cv) (Some av) v2):
-     Tarai_value (S n) (Some av) (Some bv) (Some cv) v2
-| Tarai_a_gt_b_2 n (av bv cv: Z) (v1 v2 v3 v4: Z)
-     (Hgt: av > bv)
+     (Hrec1: Tarai_value n (a-1) b c v1)
+     (Hrec2: Tarai_value n (b-1) c a v2):
+     Tarai_value (S n) a b c v2
+| Tarai_a_gt_b_2 n a b c (v1 v2 v3 v4: Z)
+     (Hgt: a > b)
      (Hle2: ~v1 <= v2)
-     (Hrec1: Tarai_value n (Some (av-1)) (Some bv) (Some cv) v1)
-     (Hrec2: Tarai_value n (Some (bv-1)) (Some cv) (Some av) v2)
-     (Hrec3: Tarai_value n (Some (cv-1)) (Some av) (Some bv) v3)
-     (Hrec4: Tarai_value n (Some v1)
-                                   (Some v2)
-                                   (Some v3) v4):
-    Tarai_value (S n) (Some av) (Some bv) (Some cv) v4.
+     (Hrec1: Tarai_value n (a-1) b c v1)
+     (Hrec2: Tarai_value n (b-1) c a v2)
+     (Hrec3: Tarai_value n (c-1) a b v3)
+     (Hrec4: Tarai_value n v1 v2 v3 v4):
+    Tarai_value (S n) a b c v4.
 
 Lemma lem_safficiency:
-  forall n a b c v, Tarai_value n a b c v -> ntarai3 n a b c = Some v.
+  forall n a b c v, Tarai_value n a b c v -> ntarai3 n (Some a) (Some b) (Some c) = Some v.
 Proof.
   intros.
   induction H.
     destruct n;
     simpl;
-    destruct (Z_le_dec av bv); auto; try contradiction.
+    destruct (Z_le_dec a b); auto; try contradiction.
 
     simpl.
     rewrite IHTarai_value1.
     rewrite IHTarai_value2.
-    destruct (Z_le_dec av bv).
-    absurd (av > bv); omega.
+    destruct (Z_le_dec a b).
+    absurd (a > b); omega.
     destruct n; simpl; destruct (Z_le_dec v1 v2); auto; contradiction.
 
     simpl.    
@@ -70,49 +68,43 @@ Proof.
     rewrite IHTarai_value2.
     rewrite IHTarai_value3.
     rewrite IHTarai_value4.
-    destruct (Z_le_dec av bv); auto; contradiction.
+    destruct (Z_le_dec a b); auto; contradiction.
 Qed.
 
 Lemma lem_necessity:
-  forall n a b c v, ntarai3 n a b c = Some v -> Tarai_value n a b c v.
+  forall n a b c v, ntarai3 n (Some a) (Some b) (Some c) = Some v -> Tarai_value n a b c v.
 Proof.
   induction n.
   intros.
   simpl in H.
-  destruct a as [av|]; [|congruence].
-  destruct b as [bv|]; [|congruence].
-  destruct (Z_le_dec av bv).
+  destruct (Z_le_dec a b).
   inversion H.
   apply Tarai_a_le_b.
   congruence.
   inversion H.
   simpl.
-  destruct a as [av|]; [|congruence].
-  destruct b as [bv|]; [|congruence].
-  destruct (Z_le_dec av bv).
   intros.
+  destruct (Z_le_dec a b).
   inversion H.
   apply Tarai_a_le_b.
   congruence.
-  destruct c as [cv|]; [|congruence].
-  intros.
-  generalize (IHn (Some (av - 1)) (Some bv) (Some cv)).
-  generalize (IHn (Some (bv - 1)) (Some cv) (Some av)).
-  generalize (IHn (Some (cv - 1)) (Some av) (Some bv)).
+  generalize (IHn (a - 1) b c).
+  generalize (IHn (b - 1) c a).
+  generalize (IHn (c - 1) a b).
   intros.
   destruct n.
-  destruct (ntarai3 0 (Some (av - 1)) (Some bv) (Some cv)) as [v1|]; [| inversion H].
-  destruct (ntarai3 0 (Some (bv - 1)) (Some cv) (Some av)) as [v2|]; [| inversion H].
+  destruct (ntarai3 0 (Some (a - 1)) (Some b) (Some c)) as [v1|]; [| inversion H].
+  destruct (ntarai3 0 (Some (b - 1)) (Some c) (Some a)) as [v2|]; [| inversion H].
   simpl in H.
   destruct (Z_le_dec v1 v2).
   apply Tarai_a_gt_b_1 with v1; auto.
   omega.
   congruence.
   inversion H.
-  destruct (ntarai3 (S n) (Some (av - 1)) (Some bv) (Some cv)) as [v1|]; [| inversion H].
-  destruct (ntarai3 (S n) (Some (bv - 1)) (Some cv) (Some av)) as [v2|]; [| inversion H].
-  destruct (ntarai3 (S n) (Some (cv - 1)) (Some av) (Some bv)) as [v3|].
-  generalize (IHn (Some v1) (Some v2) (Some v3) v H).
+  destruct (ntarai3 (S n) (Some (a - 1)) (Some b) (Some c)) as [v1|]; [| inversion H].
+  destruct (ntarai3 (S n) (Some (b - 1)) (Some c) (Some a)) as [v2|]; [| inversion H].
+  destruct (ntarai3 (S n) (Some (c - 1)) (Some a) (Some b)) as [v3|].
+  generalize (IHn v1 v2 v3 v H).
   intro.
   simpl in H.
   destruct (Z_le_dec v1 v2).
@@ -144,15 +136,15 @@ Proof.
      apply Tarai_a_gt_b_2 with v1 v2 v3; auto.
 Qed.
 
-Lemma lem1_a_gt_b_le_c : forall bv cv m, bv <= cv ->
-  exists n, Tarai_value n (Some (bv + Z_of_nat(S m))) (Some bv) (Some cv) cv.
+Lemma lem1_a_gt_b_le_c : forall b c m, b <= c ->
+  exists n, Tarai_value n (b + Z_of_nat(S m)) b c c.
 Proof.
   induction m. 
   intros.
   exists 1%nat.
   replace (Z_of_nat 1) with 1 by auto.
 
-  apply Tarai_a_gt_b_1 with bv; auto.
+  apply Tarai_a_gt_b_1 with b; auto.
   omega.
   apply Tarai_a_le_b; omega.
   apply Tarai_a_le_b; omega.
@@ -161,64 +153,64 @@ Proof.
   destruct (IHm H) as [n' Hn'].
   exists (S n').
 
-  apply Tarai_a_gt_b_1 with cv; auto.
+  apply Tarai_a_gt_b_1 with c; auto.
   rewrite inj_S. omega.
   omega.
   rewrite inj_S.
-  replace (bv + Zsucc (Z_of_nat (S m)) - 1) with (bv + Z_of_nat (S m)) by omega.
+  replace (b + Zsucc (Z_of_nat (S m)) - 1) with (b + Z_of_nat (S m)) by omega.
   auto.
 
   apply Tarai_a_le_b; omega.
 Qed. 
 
-Lemma lem_a_gt_b_le_c : forall av bv cv,  av > bv -> bv <= cv -> 
-  exists n : nat, Tarai_value n (Some av) (Some bv) (Some cv) cv.
+Lemma lem_a_gt_b_le_c : forall a b c,  a > b -> b <= c -> 
+  exists n : nat, Tarai_value n a b c c.
 Proof.
   intros. 
 
-  assert (exists m : nat, av-1-bv=Z_of_nat m). 
+  assert (exists m : nat, a-1-b=Z_of_nat m). 
   apply Z_of_nat_complete.
   omega. 
   destruct H1 as [m ?]. 
 
-  replace av with (bv + Zsucc (Z_of_nat m)) by omega.
+  replace a with (b + Zsucc (Z_of_nat m)) by omega.
   rewrite <- inj_S.
   auto using lem1_a_gt_b_le_c. 
 Qed. 
 
-Lemma lem1_a_gt_b_gt_c : forall bv cv,  bv > cv -> forall m,
-  exists n, Tarai_value n (Some (bv + Z_of_nat (S m))) (Some bv) (Some cv) (bv + Z_of_nat (S m)).
+Lemma lem1_a_gt_b_gt_c : forall b c,  b > c -> forall m,
+  exists n, Tarai_value n (b + Z_of_nat (S m)) b c (b + Z_of_nat (S m)).
 Proof.
   induction m.
   replace (Z_of_nat 1) with 1 by auto.
-  destruct (Z_le_dec (bv - 1) cv).
+  destruct (Z_le_dec (b - 1) c).
 
-  destruct (lem_a_gt_b_le_c bv cv (bv+1)) as [n0 ?]; try omega.
+  destruct (lem_a_gt_b_le_c b c (b+1)) as [n0 ?]; try omega.
   exists (S n0).
 
-  apply Tarai_a_gt_b_2 with bv cv (bv + 1); auto.
+  apply Tarai_a_gt_b_2 with b c (b + 1); auto.
   omega.
   apply Tarai_a_le_b; omega.
   apply Tarai_a_le_b; omega.
   apply Tarai_a_le_b; omega.
 
-  destruct (lem_a_gt_b_le_c (bv - 1) cv (bv + 1)) as [n0 ?]; try omega.
+  destruct (lem_a_gt_b_le_c (b - 1) c (b + 1)) as [n0 ?]; try omega.
   exists (S n0).
-  apply Tarai_a_gt_b_1 with bv; auto; try omega.
+  apply Tarai_a_gt_b_1 with b; auto; try omega.
   apply Tarai_a_le_b; omega.
 
   destruct IHm as [n0 ?].
 
   rewrite inj_S.
-  replace (bv + Zsucc (Z_of_nat (S m))) with (bv + Z_of_nat (S m) + 1) by omega.
+  replace (b + Zsucc (Z_of_nat (S m))) with (b + Z_of_nat (S m) + 1) by omega.
 
-  destruct (Z_le_dec (bv - 1) cv).
-  destruct (lem_a_gt_b_le_c (bv + Z_of_nat (S m)) cv (bv + Z_of_nat (S m) + 1)) as [n1 ?]; try omega.
+  destruct (Z_le_dec (b - 1) c).
+  destruct (lem_a_gt_b_le_c (b + Z_of_nat (S m)) c (b + Z_of_nat (S m) + 1)) as [n1 ?]; try omega.
 
   exists (S (n0 + n1)).
-  apply Tarai_a_gt_b_2 with (bv + Z_of_nat (S m)) cv  (bv + Z_of_nat (S m) + 1); auto; try omega.
+  apply Tarai_a_gt_b_2 with (b + Z_of_nat (S m)) c  (b + Z_of_nat (S m) + 1); auto; try omega.
   apply lem_n_indep.
-  replace (bv + Z_of_nat (S m) + 1 - 1) with (bv + Z_of_nat (S m)) by omega.
+  replace (b + Z_of_nat (S m) + 1 - 1) with (b + Z_of_nat (S m)) by omega.
   auto.
   apply Tarai_a_le_b; auto.
   apply Tarai_a_le_b; omega.
@@ -226,44 +218,44 @@ Proof.
   apply lem_n_indep.
   auto.
 
-  destruct (lem_a_gt_b_le_c (bv - 1) cv (bv + Z_of_nat (S m) + 1)) as [n1 ?]; try omega.
+  destruct (lem_a_gt_b_le_c (b - 1) c (b + Z_of_nat (S m) + 1)) as [n1 ?]; try omega.
   exists (S (n0 + n1)).
-  apply Tarai_a_gt_b_1 with (bv + Z_of_nat (S m)); auto; try omega.
+  apply Tarai_a_gt_b_1 with (b + Z_of_nat (S m)); auto; try omega.
   apply lem_n_indep.
-  replace (bv + Z_of_nat (S m) + 1 - 1) with (bv + Z_of_nat (S m)) by omega.
+  replace (b + Z_of_nat (S m) + 1 - 1) with (b + Z_of_nat (S m)) by omega.
   auto.
   replace (n0 + n1)%nat with (n1 + n0)%nat by omega.
   auto using lem_n_indep.
 Qed. 
 
-Lemma lem_a_gt_b_gt_c : forall av bv cv, av > bv -> bv > cv -> 
-   exists n , Tarai_value n (Some av) (Some bv) (Some cv) av.
+Lemma lem_a_gt_b_gt_c : forall a b c, a > b -> b > c -> 
+   exists n , Tarai_value n a b c a.
 Proof. 
   intros. 
-  assert (exists d: nat, av - 1 - bv=Z_of_nat d). 
+  assert (exists d: nat, a - 1 - b = Z_of_nat d). 
   apply Z_of_nat_complete. 
   omega. 
 
   destruct H1 as [m]. 
-  replace av with (bv+Z_of_nat (S m)).
+  replace a with (b + Z_of_nat (S m)).
   apply lem1_a_gt_b_gt_c; auto.
   rewrite inj_S.
   omega. 
 Qed. 
 
-Theorem tarai3_terminates : forall av bv cv,
-  exists n, exists v, Tarai_value n (Some av) (Some bv) (Some cv) v. 
+Theorem tarai3_terminates : forall a b c,
+  exists n, exists v, Tarai_value n a b c v. 
 Proof.
   intros.
-  assert (av <= bv \/ av > bv /\ bv <= cv \/ av > bv /\ bv > cv) by omega.
+  assert (a <= b \/ a > b /\ b <= c \/ a > b /\ b > c) by omega.
   destruct H as [?|[?|?]].
  
- exists 0%nat. exists bv.
+ exists 0%nat. exists b.
   apply Tarai_a_le_b; auto.
 
-  destruct (lem_a_gt_b_le_c av bv cv) as [n0 ?]; try tauto.
-  exists n0. exists cv. auto.
+  destruct (lem_a_gt_b_le_c a b c) as [n0 ?]; try tauto.
+  exists n0. exists c. auto.
 
-  destruct (lem_a_gt_b_gt_c av bv cv) as [n0 ?]; try tauto.
-  exists n0. exists av. auto.
+  destruct (lem_a_gt_b_gt_c a b c) as [n0 ?]; try tauto.
+  exists n0. exists a. auto.
 Qed.
